\begin{proposition}
\texttt{SecureFlow}, as defined, is a functor.
\end{proposition}
\begin{proof}
We are to prove the two functor laws.
\begin{enumerate}
	\item \textbf{Identity}: \texttt{fmap id = id}, where \texttt{id} is the identity function.
	\begin{lstlisting}
fmap id (Allowed a) = Allowed (id a) =
= Allowed a

fmap id Denied = Denied
	\end{lstlisting}
	Hence \texttt{fmap id = id}, as stated.
	\item \textbf{Composition}:\\ \texttt{fmap (f . g) F = fmap f (fmap g F)}
	\begin{enumerate}
		\item \texttt{F = Allowed a}:
		\begin{lstlisting}
fmap (f . g) (Allowed a) = 
= Allowed (f (g a))

fmap f (fmap g (Allowed a)) =
= fmap f (Allowed (g a)) =
= Allowed (f (g a))
		\end{lstlisting}
		\item \texttt{F = Denied}:
		\begin{lstlisting}
fmap (f . g) Denied = Denied 

fmap f (fmap g Denied) =
= fmap f Denied = Denied
		\end{lstlisting}
	\end{enumerate}
\end{enumerate}
\texttt{SecureFlow} satisfies the two functor laws, hence it is a functor.
\end{proof}